proof/TPOSR/LeftReflexivity.v
@@ -3,7 +3,9 @@ Require Import Lambda.TPOSR.Reduction.
 Require Import Lambda.TPOSR.Conv.
 Require Import Lambda.TPOSR.LiftSubst.
 Require Import Lambda.TPOSR.Env.
-Require Import Lambda.TPOSR.Types.
+Require Import Lambda.TPOSR.TypesNoDerivs.
+Require Import Lambda.TPOSR.Thinning.
+Require Import Lambda.TPOSR.CtxReduction.
 
 Set Implicit Arguments.
 
@@ -39,29 +41,32 @@ Qed.
 Hint Resolve eq_eq_l eq_eq_r coerce_coerce_l coerce_coerce_r : ecoc.
 
 Lemma ind_left_refl : 
-  (forall e u v T, e |-- u -> v : T -> e |-- u -> u : T) /\
+  (forall e u v T, e |-- u -> v : T -> e |-- u -> u : T).
+
+(* /\
   (forall e, tposr_wf e -> True) /\
-  (forall e u v s, e |-- u ~= v : s -> True) /\
-(*  e |-- u -> u : s /\ e |-- v -> v : s) /\*)
+  (forall e u v s, e |-- u ~= v : s -> 
+  e |-- u -> u : s /\ e |-- v -> v : s) /\
   (forall e u v s, e |-- u >-> v : s ->
   e |-- u -> u : s /\ e |-- v -> v : s).
 Proof.
   apply ind_tposr_wf_eq_coerce with 
   (P:=fun e u v T => fun H : e |-- u -> v : T => e |-- u -> u : T) 
   (P0:=fun e => fun H : tposr_wf e => True) 
-  (P1:=fun e u v s => fun H : e |-- u ~= v : s => True)
-
+  (P1:=fun e u v s => fun H : e |-- u ~= v : s => 
+  e |-- u -> u : s /\ e |-- v -> v : s)
   (P2:=fun e u v s => fun H : e |-- u >-> v : s =>
-  e |-- u -> u : s /\ e |-- v -> v : s) ; simpl ; intros ; intuition ; auto with coc.
+  e |-- u -> u : s /\ e |-- v -> v : s) *)
+  induction 1 ; simpl ; intros ; intuition ; auto with coc.
 
   apply tposr_prod with s1 ; auto with coc.
 
   apply tposr_abs with s1 B s2 ; auto with coc.
 
-  apply tposr_app with  A A  s1 s2 ; auto with coc.
+  apply tposr_app with  A A  s1 s2 ; eauto with coc ecoc.
 
-  apply tposr_app with A A s1 s2 ; auto with coc.
-  apply tposr_abs with s1 B s2 ; auto with coc.
+  apply tposr_app with A A s1 s2 ; eauto with coc ecoc.
+  apply tposr_abs with s1 B s2 ; eauto with coc ecoc.
   
   apply tposr_conv with A s ; auto with coc.
 
@@ -71,13 +76,13 @@ Proof.
 
   apply tposr_pi1 with s1 s2 s3 ; eauto with coc ecoc.
 
-  apply tposr_pi1 with s1 s2 s3 ; eauto with coc ecoc.
+  apply tposr_pi1 with s1 s2 s3; auto with coc ecoc.
 
   apply tposr_pi2 with s1 s2 s3 ; eauto with coc ecoc.
 
   apply tposr_pi2 with s1 s2 s3 ; eauto with coc ecoc.
-
-  apply tposr_prod with s ; auto with coc.
+Qed.
+(*  apply tposr_prod with s ; auto with coc.
 
   apply tposr_prod with s ; auto with coc.
 
@@ -85,17 +90,17 @@ Proof.
 
   apply tposr_sum with s s' ; auto with coc.
 Qed.
-
+*)
 Corollary refl_l : forall e u v T, e |-- u -> v : T -> e |-- u -> u : T.
-Proof (proj1 (ind_left_refl)).
+Proof (ind_left_refl).
 
 Corollary tposrp_refl_l : forall e A B T, tposrp e A B T -> e |-- A -> A : T.
 Proof.
   induction 1 ; auto with coc.
   apply (refl_l H).
 Qed.
-
-(*Corollary eq_refl_l : forall e u v s, e |-- u ~= v : s -> e |-- u -> u : s.
+(*
+Corollary eq_refl_l : forall e u v s, e |-- u ~= v : s -> e |-- u -> u : s.
 Proof.
   pose (proj1 (proj2 (proj2 (ind_left_refl)))).
   intros.
@@ -107,7 +112,7 @@ Proof.
   pose (proj1 (proj2 (proj2 (ind_left_refl)))).
   intros.
   destruct (a _ _ _ _ H) ; auto.
-Qed. *)
+Qed. 
 
 Corollary coerce_refl_l : forall e u v s, e |-- u >-> v : s -> e |-- u -> u : s.
 Proof.
@@ -122,5 +127,5 @@ Proof.
   intros.
   destruct (a _ _ _ _ H) ; auto.
 Qed. 
-
-Hint Resolve refl_l tposrp_refl_l coerce_refl_l coerce_refl_r : coc.
+*)
+Hint Resolve refl_l tposrp_refl_l (*eq_refl_l eq_refl_r coerce_refl_l coerce_refl_r *): coc.
