proof/TPOSR/Substitution.v
@@ -3,7 +3,7 @@ Require Import Lambda.TPOSR.Reduction.
 Require Import Lambda.TPOSR.Conv.
 Require Import Lambda.TPOSR.LiftSubst.
 Require Import Lambda.TPOSR.Env.
-Require Import Lambda.TPOSR.Types.
+Require Import Lambda.TPOSR.TypesNoDerivs.
 Require Import Lambda.TPOSR.LeftReflexivity.
 Require Import Lambda.TPOSR.Thinning.
 Require Import Lambda.TPOSR.CtxReduction.
@@ -17,41 +17,41 @@ Implicit Type s : sort.
 Implicit Types A B M N T t u v : lterm.
 Implicit Types e f g : lenv.
 
-Lemma ind_sub_weak : 
+Lemma ind_substitution : 
    (forall e t u U, e |-- t -> u : U ->
-   forall g d d' T, g |-- d -> d' : T ->
+   forall g d T, g |-- d -> d : T ->
    forall f n, sub_in_lenv d T n e f -> trunc _ n f g -> 
-   f |-- (lsubst_rec d t n) -> (lsubst_rec d' u n) : (lsubst_rec d U n)) /\
+   f |-- (lsubst_rec d t n) -> (lsubst_rec d u n) : (lsubst_rec d U n)) /\
    (forall e, tposr_wf e ->
-   forall g d d' T, g |-- d -> d' : T ->
+   forall g d T, g |-- d -> d : T ->
    forall n f, sub_in_lenv d T n e f -> trunc _ n f g -> 
    tposr_wf f) /\
    (forall e t u s, e |-- t ~= u : s ->
-   forall g d d' T, g |-- d -> d' : T ->
+   forall g d T, g |-- d -> d : T ->
    forall f n, sub_in_lenv d T n e f -> trunc _ n f g -> 
-   f |-- (lsubst_rec d t n) ~= (lsubst_rec d' u n) : s) /\
+   f |-- (lsubst_rec d t n) ~= (lsubst_rec d u n) : s) /\
    (forall e t u s, e |-- t >-> u : s ->
-   forall g d d' T, g |-- d -> d' : T ->
+   forall g d T, g |-- d -> d : T ->
    forall f n, sub_in_lenv d T n e f -> trunc _ n f g -> 
-   f |-- (lsubst_rec d t n) >-> (lsubst_rec d' u n) : s).
+   f |-- (lsubst_rec d t n) >-> (lsubst_rec d u n) : s).
 Proof.
 apply ind_tposr_wf_eq_coerce with
    (P:=fun e t u U => fun H : e |-- t -> u : U =>
-   forall g d d' T, g |-- d -> d' : T ->
+   forall g d T, g |-- d -> d : T ->
    forall f n, sub_in_lenv d T n e f -> trunc _ n f g -> 
-   f |-- (lsubst_rec d t n) -> (lsubst_rec d' u n) : (lsubst_rec d U n))
+   f |-- (lsubst_rec d t n) -> (lsubst_rec d u n) : (lsubst_rec d U n))
    (P0:= fun e => fun H : tposr_wf e =>
-   forall g d d' T, g |-- d -> d' : T ->
+   forall g d T, g |-- d -> d : T ->
    forall n f, sub_in_lenv d T n e f -> trunc _ n f g -> 
    tposr_wf f)
    (P1 := fun e t u s => fun H : e |-- t ~= u : s =>
-   forall g d d' T, g |-- d -> d' : T ->
+   forall g d T, g |-- d -> d : T ->
    forall f n, sub_in_lenv d T n e f -> trunc _ n f g -> 
-   f |-- (lsubst_rec d t n) ~= (lsubst_rec d' u n) : s)
+   f |-- (lsubst_rec d t n) ~= (lsubst_rec d u n) : s)
    (P2 := fun e t u s => fun H : e |-- t >-> u : s =>
-   forall g d d' T, g |-- d -> d' : T ->
+   forall g d T, g |-- d -> d : T ->
    forall f n, sub_in_lenv d T n e f -> trunc _ n f g -> 
-   f |-- (lsubst_rec d t n) >-> (lsubst_rec d' u n) : s);
+   f |-- (lsubst_rec d t n) >-> (lsubst_rec d u n) : s);
    simpl in |- *;
    intros; auto with coc core arith datatypes.
 
@@ -65,7 +65,7 @@ simpl in |- *.
 rewrite H3.
 rewrite simpl_lsubst; auto with coc core arith datatypes.
 apply tposr_var; auto with coc core arith datatypes.
-apply (H _ _ _ _ H0 _ _ H1) ; auto.
+apply (H _ _ _ H0 _ _ H1) ; auto.
 exists x; auto with coc core arith datatypes.
 apply nth_sub_sup with d T0 n0 e; auto with coc core arith datatypes.
 
@@ -76,14 +76,14 @@ rewrite simpl_lsubst; auto with coc core arith datatypes.
 replace x with T0.
 apply thinning_n with g; auto with coc core arith datatypes.
 subst.
-apply (H _ _ _ _ H0 _ _ H1) ; auto.
+apply (H _ _ _ H0 _ _ H1) ; auto.
 
 apply fun_item with e n; auto with coc core arith datatypes.
 apply nth_sub_eq with d f; auto with coc core arith datatypes.
 elim Heq; auto with coc core arith datatypes.
 
 apply tposr_var; auto with coc core arith datatypes.
-apply (H _ _ _ _ H0 _ _ H1) ; auto.
+apply (H _ _ _ H0 _ _ H1) ; auto.
 apply nth_sub_inf with T0 e; auto with coc core arith datatypes.
 
 apply tposr_set ; eauto with coc.
@@ -92,19 +92,19 @@ apply tposr_prop ; eauto with coc.
 
 apply tposr_prod with s1 ; eauto with coc ecoc core arith datatypes.
 
-apply tposr_abs with s1 (lsubst_rec d' B' (S n)) s2 ; eauto with coc core arith datatypes.
+apply tposr_abs with s1 (lsubst_rec d B' (S n)) s2 ; eauto with coc core arith datatypes.
 
 rewrite distr_lsubst ; auto with coc.
-apply tposr_app with (lsubst_rec d A n) (lsubst_rec d' A' n) s1 s2; eauto with coc core arith datatypes.
+apply tposr_app with (lsubst_rec d A n) (lsubst_rec d A' n) s1 s2; eauto with coc core arith datatypes.
 assert(sub_in_lenv d T (S n) (A :: e) (lsubst_rec d A n :: f)).
 apply sub_S ; auto with coc.
 assert(trunc lterm (S n) (lsubst_rec d A n :: f) g).
 apply trunc_S ; auto with coc.
-pose (H0 _ _ _ _ H3 _ _ H6 H7) ; auto with coc.
+pose (H0 _ _ _ H3 _ _ H6 H7) ; auto with coc.
 
 rewrite distr_lsubst ; auto with coc.
 rewrite distr_lsubst ; auto with coc.
-apply tposr_beta with (lsubst_rec d' A' n) s1  (lsubst_rec d' B' (S n)) s2; eauto with coc core arith datatypes.
+apply tposr_beta with (lsubst_rec d A' n) s1  (lsubst_rec d B' (S n)) s2; eauto with coc core arith datatypes.
 
 apply tposr_conv with (lsubst_rec d A n) s; eauto with coc.
 
@@ -115,20 +115,14 @@ apply tposr_sum with s1 s2; eauto with coc core arith datatypes.
 apply tposr_pair with s1 s2 s3 ; eauto with coc.
 rewrite <- distr_lsubst ; eauto with coc.
 
-pose (H _ _ _ _ H2 _ _ H3 H4).
+pose (H _ _ _ H3 _ _ H4 H5).
 apply tposr_pi1 with s1 s2 s3 ; eauto with coc.
-assert(sub_in_lenv d T (S n) (A :: e) (lsubst_rec d A n :: f)).
-apply sub_S ; auto with coc.
-assert(trunc lterm (S n) (lsubst_rec d A n :: f) g).
-apply trunc_S ; auto with coc.
-pose (H0 _ _ _ _ H4 _ _ H7 H8) ; auto with coc.
 
-pose (H2 _ _ _ _ (refl_l H4) _ _ H5 H6).
-apply tposr_pi1_red with (lsubst_rec d' A' n) s1 (lsubst_rec d' B' (S n))  s2 s3 (lsubst_rec d' v' n); eauto with coc.
+apply tposr_pi1_red with (lsubst_rec d A' n) s1 (lsubst_rec d B' (S n))  s2 s3 (lsubst_rec d v' n); eauto with coc.
 
 rewrite distr_lsubst.
 simpl.
-pose (H _ _ _ _ H2 _ _ H3 H4).
+pose (H _ _ _ H3 _ _ H4 H5).
 apply tposr_pi2 with s1 s2 s3 ; eauto with coc.
 (*assert(sub_in_lenv d T (S n) (A :: e) (lsubst_rec d A n :: f)).
 apply sub_S ; auto with coc.
@@ -139,8 +133,8 @@ destruct (H0 _ _ _ _ H2 _ _ H7 H8) ; auto with coc.
 rewrite distr_lsubst.
 simpl.
 
-pose (H2 _ _ _ _ (refl_l H4) _ _ H5 H6).
-apply tposr_pi2_red with (lsubst_rec d' A' n) s1 (lsubst_rec d' B' (S n))  s2 s3 (lsubst_rec d' u' n); eauto with coc.
+pose (H2 _ _ _ H4 _ _ H5 H6).
+apply tposr_pi2_red with (lsubst_rec d A' n) s1 (lsubst_rec d B' (S n))  s2 s3 (lsubst_rec d u' n); eauto with coc.
 (*assert(sub_in_lenv d T (S n) (A'' :: e) (lsubst_rec d A'' n :: f)).
 apply sub_S ; auto with coc.
 assert(trunc lterm (S n) (lsubst_rec d A'' n :: f) g).
@@ -151,193 +145,107 @@ inversion H0.
 inversion H1 ; subst.
 apply (wf_tposr t).
 inversion H2.
-apply wf_cons with (lsubst_rec d' A' n0) s ; apply (H _ _ _ _ H0 _ _ H7 H8).
+apply wf_cons with (lsubst_rec d A' n0) s ; apply (H _ _ _ H0 _ _ H7 H8).
 
 apply tposr_eq_tposr ; eauto with coc.
-apply tposr_eq_tposr ; eauto with coc.
-
-apply H1 ; eauto with coc.
-
-eauto with coc.
-
-
-eauto with coc.
-apply tposr_eq_trans with (lsubst_rec d X n).
-apply tposr_eq_sym.
-apply tposr_eq_tposr ; eauto with coc.
-apply tposr_eq_tposr ; eauto with coc.
-
-destruct (H _ _ _ _ H0 _ _ H1 H2).
-split ; auto with coc.
-
-
-destruct (H _ _ _ _ H1 _ _ H2 H3).
-destruct (H0 _ _ _ _ H1 _ _ H2 H3).
-destruct (H0 _ _ _ _ (refl_l H1) _ _ H2 H3).
-destruct (H _ _ _ _ (refl_l H1) _ _ H2 H3).
-split.
-apply tposr_eq_trans with (lsubst_rec d' X n) ; eauto with coc.
-eauto with coc ecoc.
 eauto with coc ecoc.
 
-destruct (H1 _ _ _ _ H2 _ _ H3 H4).
-split ; apply tposr_coerce_conv ; auto with coc.
+apply tposr_eq_trans with (lsubst_rec d X n) ; eauto with coc.
+
+pose (H _ _ _ H0 _ _ H1 H2).
+auto with coc.
+
+apply tposr_coerce_prod with s ; eauto with coc.
+
+apply tposr_coerce_sum with s s' ; eauto with coc.
+
+apply tposr_coerce_sub_l ; eauto with coc.
+
+apply tposr_coerce_sub_r ; eauto with coc.
+
 eauto with coc.
-pose (coerce_refl
-eauto with coc.
 
- ; eauto with coc ecoc.
-destruct (H0 _ _ _ _ H1 _ _ H2 H3).
-destruct (H0 _ _ _ _ (refl_l H1) _ _ H2 H3).
-destruct (H _ _ _ _ (refl_l H1) _ _ H2 H3).
-
-
-
-
-assert (tposr_wf (llift_rec 1 A' n :: f)) by (apply wf_cons with (llift_rec 1 A' n) s ; eauto with coc).
-assert (tposr_wf (llift_rec 1 A0 n :: f)) by (apply wf_cons with (llift_rec 1 A0 n) s ; eauto with coc).
-apply tposr_coerce_prod with s ; auto with coc.
-
-assert (tposr_wf (llift_rec 1 A' n :: f)) by (apply wf_cons with (llift_rec 1 A' n) s ; eauto with coc).
-assert (tposr_wf (llift_rec 1 A0 n :: f)) by (apply wf_cons with (llift_rec 1 A0 n) s ; eauto with coc).
-apply tposr_coerce_sum with s s' ; auto with coc.
-
-assert (tposr_wf (llift_rec 1 U n :: f)) by (apply wf_cons with (llift_rec 1 U n) set ; eauto with coc).
-apply tposr_coerce_sub_l ; auto with coc.
-
-assert (tposr_wf (llift_rec 1 U' n :: f)) by (apply wf_cons with (llift_rec 1 U' n) set ; eauto with coc).
-apply tposr_coerce_sub_r ; auto with coc.
-
-apply tposr_coerce_trans with (llift_rec 1 B n) ; auto with coc.
+apply tposr_coerce_trans with (lsubst_rec d B n) ; eauto with coc.
 Qed.
 
-
-Theorem tposr_sub : forall g d d' t, g |-- d -> d' : t ->
+Corollary substitution_tposr_n : forall g d t, g |-- d -> d : t ->
    forall e u v U, e |-- u -> v : U ->
    forall f n, sub_in_lenv d t n e f -> trunc _ n f g -> 
-   f |-- (lsubst_rec d u n) -> (lsubst_rec d' v n) : (lsubst_rec d U n).
-Admitted.
+   f |-- (lsubst_rec d u n) -> (lsubst_rec d v n) : (lsubst_rec d U n).
+Proof.
+  intros.
+  eapply (proj1 (ind_substitution)) ; eauto with coc.
+Qed.
 
-Theorem tposr_wf_sub : forall g d d' t, g |-- d -> d' : t ->
-   forall e, tposr_wf e -> forall f n, sub_in_lenv d t n e f -> tposr_wf f.
-Admitted.
+Corollary substitution_tposr_wf_n : forall g d t, g |-- d -> d : t ->
+   forall e, tposr_wf e -> forall f n, sub_in_lenv d t n e f -> 
+   trunc _ n f g -> tposr_wf f.
+Proof.
+  intros.
+  eapply (proj1 (proj2 (ind_substitution))) ; eauto with coc.
+Qed.
 
-Theorem tposr_coerce_sub : forall g d d' t, g |-- d -> d' : t ->
+Corollary substitution_eq_n : forall g d t, g |-- d -> d : t ->
+   forall e u v s, e |-- u ~= v : s ->
+   forall f n, sub_in_lenv d t n e f -> trunc _ n f g -> 
+   f |-- (lsubst_rec d u n) ~= (lsubst_rec d v n) : s.
+Proof.
+  intros.
+  eapply (proj1 (proj2 (proj2 (ind_substitution)))) ; eauto with coc.
+Qed.
+
+Corollary substitution_coerce_n : forall g d t, g |-- d -> d : t ->
    forall e u v s, e |-- u >-> v : s ->
    forall f n, sub_in_lenv d t n e f -> trunc _ n f g -> 
-   f |-- (lsubst_rec d u n) >-> (lsubst_rec d' v n) : s.
-Admitted.
+   f |-- (lsubst_rec d u n) >-> (lsubst_rec d v n) : s.
+Proof.
+  intros.
+  eapply (proj2 (proj2 (proj2 (ind_substitution)))) ; eauto with coc.
+Qed.
 
-Theorem substitution : forall e t u v U, (t :: e) |-- u -> v : U ->
-  forall d d', e |-- d -> d' : t -> e |-- (lsubst d u) -> (lsubst d' v) : (lsubst d U).
-Admitted.
+Corollary substitution : forall e t u v U, (t :: e) |-- u -> v : U ->
+  forall d, e |-- d -> d : t -> e |-- (lsubst d u) -> (lsubst d v) : (lsubst d U).
+Proof.
+  intros ; unfold lsubst ; eapply substitution_tposr_n ; eauto with coc.
+Qed.
 
-Corollary tposrp_substitution_aux : forall G u v U, G |-- u -+> v : U -> forall t e, G = (t :: e) ->
-  forall d d', e |-- d -> d' : t -> e |-- (lsubst d u) -+> (lsubst d' v) : (lsubst d U).
+Corollary substitution_eq : 
+   forall e t u v s, t :: e |-- u ~= v : s ->
+   forall d, e |-- d -> d : t ->
+   e |-- (lsubst d u) ~= (lsubst d v) : s.
+Proof.
+  intros ; unfold lsubst ; eapply substitution_eq_n ; eauto with coc.
+Qed.
+
+Corollary substitution_coerce : 
+   forall e t u v s, t :: e |-- u >-> v : s ->
+   forall d, e |-- d -> d : t ->
+   e |-- (lsubst d u) >-> (lsubst d v) : s.
+Proof.
+  intros ; unfold lsubst ; eapply substitution_coerce_n ; eauto with coc.
+Qed.
+
+Corollary substitution_tposrp_aux : forall G u v U, G |-- u -+> v : U -> forall t e, G = (t :: e) ->
+  forall d, e |-- d -> d : t -> e |-- (lsubst d u) -+> (lsubst d v) : (lsubst d U).
 Proof.
   induction 1 ; simpl ; intros; subst ; eauto with coc ecoc.
   apply tposrp_tposr.
   apply substitution with t ; auto.
 Qed.
 
-Corollary tposrp_substitution : forall t e u v U, t :: e |-- u -+> v : U -> 
-  forall d d', e |-- d -> d' : t -> e |-- (lsubst d u) -+> (lsubst d' v) : (lsubst d U).
+Corollary substitution_tposrp : forall t e u v U, t :: e |-- u -+> v : U -> 
+  forall d, e |-- d -> d : t -> e |-- (lsubst d u) -+> (lsubst d v) : (lsubst d U).
 Proof.
   intros.
-  eapply tposrp_substitution_aux  ; eauto with coc.
+  eapply substitution_tposrp_aux  ; eauto with coc.
 Qed.
 
 Corollary substitution_sorted : forall e t u v s, (t :: e) |-- u -> v : Srt_l s ->
-  forall d d', e |-- d -> d' : t -> e |-- (lsubst d u) -> (lsubst d' v) : Srt_l s.
+  forall d, e |-- d -> d : t -> e |-- (lsubst d u) -> (lsubst d v) : Srt_l s.
 Proof.
   intros.
   change (Srt_l s) with (lsubst d (Srt_l s)).
   apply substitution with t ; auto.
 Qed.
 
-Corollary substitution_eq_aux : forall G u v s, G |-- u ~= v : s -> forall e t, G = (t :: e) ->
-  forall d, e |-- d -> d : t -> e |-- (lsubst d u) ~= (lsubst d v) : s.
-Proof.
-  induction 1 ; simpl ; intros ; eauto with coc.
-  subst.
-  apply tposr_eq_tposr.
-  apply substitution_sorted with t ; auto.
-  apply tposr_eq_trans with (lsubst d X) ; eauto with coc.
-Qed.
-
-Corollary substitution_eq : forall t e u v s, t :: e |-- u ~= v : s -> 
-  forall d, e |-- d -> d : t -> e |-- (lsubst d u) ~= (lsubst d v) : s.
-Proof.
-  intros ; eapply substitution_eq_aux ; eauto with coc.
-Qed.
-
-Corollary substitution_coerce : forall t e u v s, t :: e |-- u >-> v : s -> 
-  forall d d', e |-- d -> d' : t -> e |-- (lsubst d u) >-> (lsubst d' v) : s.
-Proof.
-  intros.
-  unfold lsubst ; eapply tposr_coerce_sub ; auto with coc.
-  apply H0.
-  apply H.
-Qed.
-
-Lemma typ_sub_weak : forall g (d : term) t, g |-- d : t ->
-   forall e u (U : term), e |-- u : U ->
-   forall f n, sub_in_env d t n e f -> trunc _ n f g -> 
-   f |-- (subst_rec d u n) : (subst_rec d U n).
-Proof.
-  intros g d t H.
-  exact (proj1 (ind_sub_weak H)).
-Qed.
-
-Lemma coerce_sub_weak : forall g (d : term) t, g |-- d : t ->
-   forall e T U s, e |-- T >> U : s ->
-   forall f n, sub_in_env d t n e f -> trunc _ n f g -> 
-   f |-- (subst_rec d T n) >> (subst_rec d U n) : s.
-Proof.
-  intros g d t H.
-  exact (proj1 (proj2 (ind_sub_weak H))).
-Qed.
-
-Lemma jeq_sub_weak : forall g (d : term) t, g |-- d : t ->
-   forall e U V T, e |-- U = V : T ->
-   forall f n, sub_in_env d t n e f -> trunc _ n f g -> 
-   f |-- (subst_rec d U n) = (subst_rec d V n) : (subst_rec d T n).
-Proof.
-  intros g d t H.
-  exact (proj2 (proj2 (ind_sub_weak H))).
-Qed.
-
-Theorem substitution : forall e t u U, (t :: e) |-- u : U ->
-  forall d, e |-- d : t -> e |-- (subst d u) : (subst d U).
-Proof.
-intros.
-unfold subst in |- *.
-destruct (ind_sub_weak H0). 
-apply H1 with (t :: e) ; auto with coc core arith datatypes.
-Qed.
-
-Theorem substitution_coerce : forall e t T (U : term) s,
-  (t :: e) |-- T >> U : s ->
-  forall d, e |-- d : t -> e |-- (subst d T) >> (subst d U) : s.
-Proof.
-intros.
-unfold subst in |- *.
-destruct (ind_sub_weak H0). 
-destruct H2.
-apply H2 with (t :: e); auto with coc core arith datatypes.
-Qed.
-
-Theorem substitution_jeq : forall e t U V T,
-  (t :: e) |-- U = V : T ->
-  forall d, e |-- d : t -> e |-- (subst d U) = (subst d V) : subst d T.
-Proof.
-intros.
-unfold subst in |- *.
-destruct (ind_sub_weak H0). 
-destruct H2.
-apply H3 with (t :: e); auto with coc core arith datatypes.
-Qed.
-
-Hint Resolve substitution substitution_coerce substitution_jeq : coc.
-
-*)
+Hint Resolve substitution substitution_coerce substitution_eq substitution_tposrp : ecoc.
