proof/TPOSR/Thinning.v
@@ -3,8 +3,8 @@ Require Import Lambda.TPOSR.Reduction.
 Require Import Lambda.TPOSR.LiftSubst.
 Require Import Lambda.TPOSR.Env.
 Require Import Lambda.TPOSR.Conv.
-Require Import Lambda.TPOSR.Types.
-Require Import Lambda.TPOSR.LeftReflexivity.
+Require Import Lambda.TPOSR.TypesNoDerivs.
+(*Require Import Lambda.TPOSR.LeftReflexivity.*)
 
 Set Implicit Arguments.
 
@@ -89,11 +89,10 @@ apply tposr_pair with s1 s2 s3 ; auto with coc.
 rewrite <- distr_llift_lsubst ; auto with coc.
 
 apply tposr_pi1 with s1 s2 s3 ; auto with coc.
-apply H0 ; eauto with coc .
+apply H1 ; eauto with coc.
 apply wf_cons with (llift_rec 1 A0 n) s1 ; eauto with coc.
 
-assert (tposr_wf (llift_rec 1 A0 n :: f)) by (apply wf_cons with (llift_rec 1 A0 n) s1 ; eauto with coc).
-assert (tposr_wf (llift_rec 1 A'' n :: f)) by (apply wf_cons with (llift_rec 1 A'' n) s1 ; eauto with coc).
+assert (tposr_wf (llift_rec 1 A0 n :: f)) by (apply wf_cons with (llift_rec 1 A' n) s1 ; eauto with coc).
 apply tposr_pi1_red with (llift_rec 1 A' n) s1 (llift_rec 1 B' (S n))  s2 s3 (llift_rec 1 v' n); auto with coc.
 
 assert (tposr_wf (llift_rec 1 A0 n :: f)) by (apply wf_cons with (llift_rec 1 A0 n) s1 ; eauto with coc).
@@ -101,13 +100,13 @@ rewrite distr_llift_lsubst.
 simpl.
 apply tposr_pi2 with s1 s2 s3 ; auto with coc.
 
-assert (tposr_wf (llift_rec 1 A0 n :: f)) by (apply wf_cons with (llift_rec 1 A0 n) s1 ; eauto with coc).
-assert (tposr_wf (llift_rec 1 A'' n :: f)) by (apply wf_cons with (llift_rec 1 A'' n) s1 ; eauto with coc).
+assert (tposr_wf (llift_rec 1 A0 n :: f)) by (apply wf_cons with (llift_rec 1 A' n) s1 ; eauto with coc).
 rewrite distr_llift_lsubst.
 simpl.
 apply tposr_pi2_red with (llift_rec 1 A' n) s1 (llift_rec 1 B' (S n))  s2 s3 (llift_rec 1 u' n); auto with coc.
 
 apply tposr_eq_trans with (llift_rec 1 X n) ; auto with coc.
+
 
 assert (tposr_wf (llift_rec 1 A' n :: f)) by (apply wf_cons with (llift_rec 1 A' n) s ; eauto with coc).
 assert (tposr_wf (llift_rec 1 A0 n :: f)) by (apply wf_cons with (llift_rec 1 A0 n) s ; eauto with coc).
